Rename HML datatype constructors

HML/HML.thy
@@ -3,16 +3,16 @@ theory HML
 begin
 
 datatype 
-  ('act, 'i) HML =
-    HML_true |
-    HML_poss 'act "('act, 'i) HML" |
-    HML_silent "('act, 'i) HML" |
-    HML_internal "('act, 'i) HML" |
-    HML_conj "'i set" "'i \<Rightarrow> ('act, 'i) HML_neg"
+  ('act, 'i) hml =
+    TT |
+    Obs 'act "('act, 'i) hml" |
+    Silent "('act, 'i) hml" |
+    Internal "('act, 'i) hml" |
+    Conj "'i set" "'i \<Rightarrow> ('act, 'i) hml_conjunct"
 and
-  ('act, 'i) HML_neg =
-    HML_just "('act, 'i) HML" |
-    HML_not "('act, 'i) HML"
+  ('act, 'i) hml_conjunct =
+    Pos "('act, 'i) hml" |
+    Neg "('act, 'i) hml"
 
 
 
@@ -20,26 +20,26 @@ context LTS_Tau
 begin
 
 function
-      hml_models     :: "('a, 's) HML     \<Rightarrow> 's \<Rightarrow> bool" ("_ \<Turnstile> _" 60) 
-  and hml_neg_models :: "('a, 's) HML_neg \<Rightarrow> 's \<Rightarrow> bool"
+      hml_models     :: "('a, 's) hml     \<Rightarrow> 's \<Rightarrow> bool" ("_ \<Turnstile> _" 60) 
+  and hml_neg_models :: "('a, 's) hml_conjunct \<Rightarrow> 's \<Rightarrow> bool"
 where
-  "(HML_true         \<Turnstile> _) = True" |
-  "((HML_poss a \<phi>)   \<Turnstile> p) = (\<exists>p'. p \<mapsto> a p' \<and> (\<phi> \<Turnstile> p'))" |
-  "((HML_silent \<phi>)   \<Turnstile> p) = (\<exists>p'. p \<Zsurj> p' \<and> (\<phi> \<Turnstile> p'))" |
-  "((HML_internal \<phi>) \<Turnstile> p) = ((\<exists>p'. p \<mapsto> \<tau> p' \<and> (\<phi> \<Turnstile> p')) \<or> (\<phi> \<Turnstile> p))" |
-  "((HML_conj I \<psi>s)  \<Turnstile> p) = (\<forall>i \<in> I. hml_neg_models (\<psi>s i) p)" |
+  "(TT           \<Turnstile> _) = True" |
+  "((Obs a \<phi>)    \<Turnstile> p) = (\<exists>p'. p \<mapsto> a p' \<and> (\<phi> \<Turnstile> p'))" |
+  "((Silent \<phi>)   \<Turnstile> p) = (\<exists>p'. p \<Zsurj> p' \<and> (\<phi> \<Turnstile> p'))" |
+  "((Internal \<phi>) \<Turnstile> p) = ((\<exists>p'. p \<mapsto> \<tau> p' \<and> (\<phi> \<Turnstile> p')) \<or> (\<phi> \<Turnstile> p))" |
+  "((Conj I \<psi>s)  \<Turnstile> p) = (\<forall>i \<in> I. hml_neg_models (\<psi>s i) p)" |
 
-  "(hml_neg_models (HML_just \<phi>) p) = (\<phi> \<Turnstile> p)" |
-  "(hml_neg_models (HML_not \<phi>) p) = (\<not>(\<phi> \<Turnstile> p))"
-  by (metis HML.exhaust HML_neg.exhaust sumE surj_pair, auto)
+  "(hml_neg_models (Pos \<phi>) p) = (\<phi> \<Turnstile> p)" |
+  "(hml_neg_models (Neg \<phi>) p) = (\<not>(\<phi> \<Turnstile> p))"
+  by (metis hml.exhaust hml_conjunct.exhaust sumE surj_pair, auto)
             
-inductive_set hml_models_wf_arg_space :: "(('a, 's) HML \<times> 's, ('a, 's) HML_neg \<times> 's) sum rel" where
-                         "(Inl (\<phi>, x), Inl (HML_poss   a \<phi>, p)) \<in> hml_models_wf_arg_space" |
-                         "(Inl (\<phi>, x), Inl (HML_silent   \<phi>, p)) \<in> hml_models_wf_arg_space" |
-                         "(Inl (\<phi>, x), Inl (HML_internal \<phi>, p)) \<in> hml_models_wf_arg_space" |
-  "i \<in> I \<Longrightarrow> \<psi> = \<psi>s i \<Longrightarrow> (Inr (\<psi>, p), Inl (HML_conj  I \<psi>s, p)) \<in> hml_models_wf_arg_space" |
-                         "(Inl (\<phi>, p), Inr (HML_just     \<phi>, p)) \<in> hml_models_wf_arg_space" |
-                         "(Inl (\<phi>, p), Inr (HML_not      \<phi>, p)) \<in> hml_models_wf_arg_space"
+inductive_set hml_models_wf_arg_space :: "(('a, 's) hml \<times> 's, ('a, 's) hml_conjunct \<times> 's) sum rel" where
+                          "(Inl (\<phi>, x), Inl (Obs    a \<phi>, p)) \<in> hml_models_wf_arg_space" |
+                          "(Inl (\<phi>, x), Inl (Silent   \<phi>, p)) \<in> hml_models_wf_arg_space" |
+                          "(Inl (\<phi>, x), Inl (Internal \<phi>, p)) \<in> hml_models_wf_arg_space" |
+  "i \<in> I \<Longrightarrow> \<psi> = \<psi>s i \<Longrightarrow> (Inr (\<psi>, p), Inl (Conj  I \<psi>s, p)) \<in> hml_models_wf_arg_space" |
+                          "(Inl (\<phi>, p), Inr (Pos      \<phi>, p)) \<in> hml_models_wf_arg_space" |
+                          "(Inl (\<phi>, p), Inr (Neg      \<phi>, p)) \<in> hml_models_wf_arg_space"
 
 lemma wf_hml_models_wf_arg_space: "wf hml_models_wf_arg_space"
   unfolding wf_def
@@ -49,43 +49,43 @@ proof safe
 
   then show "P \<phi>sOr\<psi>s"
   proof (induct \<phi>sOr\<psi>s)
-    fix \<phi>s :: "('a, 's) HML \<times> 's"
+    fix \<phi>s :: "('a, 's) hml \<times> 's"
     obtain \<phi> and sl where "\<phi>s = (\<phi>, sl)" by fastforce
 
-    fix \<psi>s :: "('a, 's) HML_neg \<times> 's"
+    fix \<psi>s :: "('a, 's) hml_conjunct \<times> 's"
     obtain \<psi> and sr where "\<psi>s = (\<psi>, sr)" by fastforce
 
     show "P (Inl \<phi>s)" and "P (Inr \<psi>s)"
       unfolding \<open>\<phi>s = (\<phi>, sl)\<close> and \<open>\<psi>s = (\<psi>, sr)\<close>
       using \<open>\<forall>x. (\<forall>y. (y, x) \<in> hml_models_wf_arg_space \<longrightarrow> P y) \<longrightarrow> P x\<close>
     proof (induct \<phi> and \<psi> arbitrary: sl and sr)
-      case HML_true
+      case TT
       then show ?case
-        by (smt (verit) HML.distinct(1) HML.distinct(3) HML.distinct(5) HML.distinct(7) Inl_inject Pair_inject hml_models_wf_arg_space.simps sum.distinct(1))
+        by (smt (verit) hml.distinct(1) hml.distinct(3) hml.distinct(5) hml.distinct(7) Inl_inject Pair_inject hml_models_wf_arg_space.simps sum.distinct(1))
     next
-      case (HML_poss x1 x2)
+      case (Obs x1 x2)
       then show ?case
-        by (smt (verit) HML.distinct(11) HML.distinct(13) HML.distinct(9) HML.inject(1) Inl_inject Pair_inject hml_models_wf_arg_space.simps sum.distinct(1))
+        by (smt (verit) hml.distinct(11) hml.distinct(13) hml.distinct(9) hml.inject(1) Inl_inject Pair_inject hml_models_wf_arg_space.simps sum.distinct(1))
     next
-      case (HML_silent x)
+      case (Silent x)
       then show ?case
-        by (smt (verit) HML.distinct(15) HML.distinct(17) HML.distinct(9) HML.inject(2) Inl_inject Pair_inject hml_models_wf_arg_space.simps sum.distinct(1))
+        by (smt (verit) hml.distinct(15) hml.distinct(17) hml.distinct(9) hml.inject(2) Inl_inject Pair_inject hml_models_wf_arg_space.simps sum.distinct(1))
     next
-      case (HML_internal x)
+      case (Internal x)
       then show ?case
-        by (smt (verit) HML.distinct(11) HML.distinct(15) HML.distinct(19) HML.inject(3) Inl_inject Pair_inject hml_models_wf_arg_space.simps sum.distinct(1))
+        by (smt (verit) hml.distinct(11) hml.distinct(15) hml.distinct(19) hml.inject(3) Inl_inject Pair_inject hml_models_wf_arg_space.simps sum.distinct(1))
     next
-      case (HML_conj x1 x2)
+      case (Conj x1 x2)
       then show ?case
-        by (smt (verit) HML.distinct(13) HML.distinct(17) HML.distinct(19) HML.inject(4) Inl_inject Pair_inject hml_models_wf_arg_space.simps range_eqI sum.distinct(1))
+        by (smt (verit) hml.distinct(13) hml.distinct(17) hml.distinct(19) hml.inject(4) Inl_inject Pair_inject hml_models_wf_arg_space.simps range_eqI sum.distinct(1))
     next
-      case (HML_just x)
+      case (Pos x)
       then show ?case
-        by (smt (verit) HML_neg.distinct(1) HML_neg.inject(1) Inr_inject Pair_inject hml_models_wf_arg_space.simps sum.distinct(1))
+        by (smt (verit) hml_conjunct.distinct(1) hml_conjunct.inject(1) Inr_inject Pair_inject hml_models_wf_arg_space.simps sum.distinct(1))
     next
-      case (HML_not x)
+      case (Neg x)
       then show ?case
-        by (smt (verit) HML_neg.distinct(2) HML_neg.inject(2) Inr_inject Pair_inject hml_models_wf_arg_space.simps sum.distinct(1))
+        by (smt (verit) hml_conjunct.distinct(2) hml_conjunct.inject(2) Inr_inject Pair_inject hml_models_wf_arg_space.simps sum.distinct(1))
     qed
   qed
 qed
